@prefix rdf: <http://www.w3.org/1999/02/22-rdf-syntax-ns#> .
@prefix rdfs: <http://www.w3.org/2000/01/rdf-schema#> .
@prefix xsd: <http://www.w3.org/2001/XMLSchema#> .
@prefix owl: <http://www.w3.org/2002/07/owl#> .
@prefix vcs: <tag:stardog:api:versioning:> .
@prefix prov: <http://www.w3.org/ns/prov#> .

vcs:Version a owl:Class ;
	rdfs:comment "Represents a version in the database. Every commit in the database creates a new version. Each version has a committer (prov:wasAttributedTo), a commit time (prov:generatedAtTime) and optionally a commit message (rdfs:comment). There is a link to the previous version (prov:wasRevisionOf) if this is not the first version. There will be one or more updates (vcs:update) for each update." ;
	rdfs:subClassOf prov:Entity , [ 
		rdf:type owl:Restriction ;
		owl:onProperty prov:wasAttributedTo ;
		owl:cardinality 1
	] , [ 
		rdf:type owl:Restriction ;
		owl:onProperty prov:wasAttributedTo ;
		owl:allValuesFrom prov:Person
	] , [ 
		rdf:type owl:Restriction ;
		owl:onProperty prov:generatedAtTime ;
		owl:cardinality 1
	] , [ 
		rdf:type owl:Restriction ;
		owl:onProperty prov:wasRevisionOf ;
		owl:maxCardinality 1
	] , [ 
		rdf:type owl:Restriction ;
		owl:onProperty prov:wasRevisionOf ;
		owl:allValuesFrom vcs:Version
	] , [ 
		rdf:type owl:Restriction ;
		owl:onProperty vcs:updates ;
		owl:minCardinality 1
	] .

vcs:HeadVersion a owl:Class ;
	rdfs:comment "Final version of a database. There is only one instance of this class in each versioning history. The instance of this class is updated after every commit." .

vcs:Updates a owl:Class ;
	rdfs:comment "Represents the changes to a specific named graph in a commit. All the changes to a named graph is grouped under one instance of this class for each commit. Triples added to (removed from) the specified named graph in this version is stored under the named graph pointed by the vcs:additions (vcs:removals) property. If there were no additions or no removals in a commit then the corresponding property will not exist." ;
	rdfs:subClassOf [ 
		rdf:type owl:Restriction ;
		owl:onProperty vcs:graph ;
		owl:cardinality 1
	] , [ 
		rdf:type owl:Restriction ;
		owl:onProperty vcs:additions ;
		owl:maxCardinality 1
	] , [ 
		rdf:type owl:Restriction ;
		owl:onProperty vcs:removals ;
		owl:maxCardinality 1
	] .

vcs:NamedGraph a owl:Class ;
	rdfs:comment "Represents a named graph in the versioning metadata" .

vcs:updates a owl:ObjectProperty ;
	rdfs:comment "Links to an update instance." ;
	rdfs:domain vcs:Version ;
	rdfs:range vcs:Updates .

vcs:graph a owl:ObjectProperty ;
	rdfs:comment "Link to the named graph modified by a commit." ;
	rdfs:domain vcs:Updates ;
	rdfs:range vcs:NamedGraph .

vcs:additions a owl:ObjectProperty ;
	rdfs:comment "Link to the named graph that stores the triples added by a commit." ;
	rdfs:domain vcs:Updates ;
	rdfs:range vcs:NamedGraph .

vcs:removals a owl:ObjectProperty ;
	rdfs:comment "Link to the named graph that stores the triples removed by a commit." ;
	rdfs:domain vcs:Updates ;
	rdfs:range vcs:NamedGraph .

vcs:tag a owl:DatatypeProperty ;
	rdfs:comment "Links a version to the label of the tag created for that version." ;
	rdfs:domain vcs:Version ;
	rdfs:range xsd:string .

vcs:Tag a owl:Class ;
	rdfs:comment "Represents a tag created for a version. Each tag has a creator (prov:wasAttributedTo) and a creation time (prov:generatedAtTime). The label of the tag is specified by the rdfs:label which matches the label used by the vcs:tag property." ;
	rdfs:subClassOf prov:Entity , [ 
		rdf:type owl:Restriction ;
		owl:onProperty prov:wasAttributedTo ;
		owl:cardinality 1
	] , [ 
		rdf:type owl:Restriction ;
		owl:onProperty prov:wasAttributedTo ;
		owl:allValuesFrom prov:Person
	] , [ 
		rdf:type owl:Restriction ;
		owl:onProperty prov:generatedAtTime ;
		owl:cardinality 1
	] .
